Tealeaves/Examples/STLC/Simplification.v
@@ -1,12 +1,522 @@
 From Tealeaves Require Export
   Examples.STLC.Syntax.
 
+Import LN.Notations.
 Import STLC.Syntax.Notations.
+
 #[local] Notation "'P'" := pure.
 #[local]  Notation "'BD'" := binddt.
 #[local] Open Scope tealeaves_scope.
 
+Section section.
+  Context {E : Type} {T : Type -> Type} `{Mapdt E T}.
+
+  Lemma Forall_ctx_to_foldMapd :
+    forall {A t} (f: E * A -> Prop),
+      Forall_ctx f t = foldMapd f t.
+  Proof.
+    reflexivity.
+  Qed.
+  Lemma foldMapd_to_Forall_ctx :
+    forall {A t} (f: E * A -> Prop),
+      foldMapd f t = Forall_ctx f t.
+  Proof.
+    reflexivity.
+  Qed.
+
+  Lemma exists_false_false
+          `{DecoratedTraversableFunctor E T}:
+    forall {A} (t: T A),
+      foldMapd (op := Monoid_op_or) (unit := Monoid_unit_false)
+        (const False) t = False.
+  Proof.
+    intros.
+    rewrite foldMapd_through_toctxlist.
+    unfold compose. induction (toctxlist t).
+    - reflexivity.
+    - cbn. rewrite IHe. do 2 unfold transparent tcs. propext;
+                        intuition.
+  Qed.
+
+End section.
+
+Lemma binddt_ret:
+  forall {W : Type} {T G : Type -> Type}
+    `{DecoratedTraversableMonad W T}
+    `{Applicative G},
+      forall (A B : Type) (f : W * A -> G (T B)) (a: A),
+        binddt f (ret a) = f (Ƶ, a).
+Proof.
+  intros.
+  compose near a.
+  rewrite kdtm_binddt0.
+  reflexivity.
+Qed.
+(*
 Ltac simplify := simplify_with_simplify_binddt term ltac:(fun unit => cbn).
+ *)
+
+Ltac normalize_fns :=
+  match goal with
+  | |- context[?f ∘ id] =>
+      change (f ∘ id) with f
+  | |- context[(id ∘ ?f)] =>
+      change (id ∘ f) with f
+  end.
+
+Ltac normalize_id :=
+  match goal with
+  | |- context[id ?t] =>
+      change (id t) with t
+  end.
+
+Ltac push_preincr_into_fn :=
+  match goal with
+  | |- context[(?g ∘ ?f) ⦿ ?w] =>
+      rewrite (preincr_assoc g f w)
+  | |- context[extract ⦿ ?w] =>
+      rewrite (extract_preincr w)
+  end.
+
+Ltac simplify_post_binddt_ret :=
+  match goal with
+  | |- context[map (F := const ?X) ?f ∘ ?g] =>
+      change (map (F := const ?X) ?f ∘ ?g) with g
+  | |- context[map (F := const ?X) ?f] =>
+      rewrite map_const_rw;
+      try normalize_id
+  | |- context[(?f ∘ extract) (?w, ?a)] =>
+      change ((f ∘ extract) (w, a)) with (f a)
+  | |- context[extract (?w, ?a)] =>
+      change (extract (w, a)) with a
+  | |- context[(?f ∘ ret (T := ?T) ?a)] =>
+      change (f ∘ ret (T := T) a) with (f (ret a))
+  end.
+
+Ltac simplify_binddt_ret :=
+  match goal with
+  | |- context[binddt (T := ?T) ?f (?rtn ?t)] =>
+      change (rtn t) with (ret (T := T) t);
+      rewrite binddt_ret;
+      repeat simplify_post_binddt_ret
+  end.
+
+Ltac simplify_binddt_core :=
+  match goal with
+  | |- context[binddt (W := ?W) (T := ?T)
+                (H := ?H) (H0 := ?H0) (H1 := ?H1)
+                (U := ?U) (G := ?G) ?f ?t] =>
+      let e := constr:(binddt (W := W) (T := T) (U := U) (G := G)
+                         (H := H) (H0 := H0) (H1 := H1)
+                         f t) in
+      let e' := eval cbn in e in
+        debug "simplify_binddt_core|change";
+        progress (change e with e' in *)
+  end.
+
+Ltac simplify_binddt :=
+   (simplify_binddt_ret
+    (* || cbn; repeat push_preincr_into_fn *)
+    || simplify_binddt_core; repeat push_preincr_into_fn).
+
+Ltac simplify_mapdt :=
+  match goal with
+  | |- context[mapdt (T := ?T) ?f (ret ?t)] =>
+      idtac "mapdt_ret should be called here"
+  | |- context[mapdt (T := ?T)] =>
+      rewrite (mapdt_to_binddt (T := T));
+      simplify_binddt;
+      repeat rewrite <- (mapdt_to_binddt (T := T))
+  end.
+
+Ltac simplify_bindt :=
+  match goal with
+  | |- context[bindt (T := ?T) ?f (ret ?t)] =>
+      idtac "bindt_ret should be called here"
+  | |- context[bindt (T := ?T)] =>
+      rewrite (bindt_to_binddt (T := T));
+      simplify_binddt;
+      repeat rewrite <- (bindt_to_binddt (T := T))
+  end.
+
+Ltac simplify_bindd :=
+  match goal with
+  | |- context[bindd (T := ?T) ?f (ret ?t)] =>
+      idtac "bindt_ret should be called here"
+  | |- context[bindd (T := ?T)] =>
+      rewrite (bindd_to_binddt (T := T));
+      simplify_binddt;
+      repeat rewrite <- (bindd_to_binddt (T := T));
+      repeat simplify_applicative_I
+  end.
+
+Ltac simplify_bind :=
+  match goal with
+  | |- context[bind (T := ?T) ?f (ret ?t)] =>
+      idtac "bind_ret should be called here"
+  | |- context[bind (T := ?T)] =>
+      rewrite (bind_to_bindd (T := T));
+      simplify_bindd;
+      repeat rewrite <- (bind_to_bindd (T := T))
+  end.
+
+Ltac simplify_traverse :=
+  match goal with
+  | |- context[traverse (T := ?T) ?f (ret ?t)] =>
+      idtac "traverse_ret should be called here"
+  | |- context[traverse (T := ?T) (G := ?G) ?f ?t] =>
+      rewrite (traverse_to_bindt (T := T) (G := G) f);
+      (* Don't simplify this yet, we need it for: rewrite <-
+      (* in case applicative is constant *)
+      repeat change (map (F := const ?M) ?f ∘ ?g) with g;
+      *)
+      repeat simplify_bindt;
+      repeat rewrite <- (traverse_to_bindt (T := T))
+             (*
+      (* in case applicative is constant *)
+      repeat change (map (F := const ?M) ?f ∘ ?g) with g;
+      *)
+end.
+
+Ltac simplify_foldMapd :=
+  match goal with
+  | |- context[foldMapd (T := ?T) (M := ?M) (op := ?op) (unit := ?unit)] =>
+      rewrite foldMapd_to_mapdt1;
+      simplify_mapdt;
+      repeat rewrite <- foldMapd_to_mapdt1;
+      repeat simplify_applicative_const;
+      (* ^ above step creates some ((Ƶ ● m) ● n) *)
+      repeat simplify_monoid_units
+  end.
+
+Ltac simplify_foldMap_post :=
+  repeat simplify_applicative_const;
+      (* ^ above step creates some ((Ƶ ● m) ● n) *)
+  repeat simplify_monoid_units;
+  repeat change (const ?x ?y) with x.
+
+Ltac simplify_foldMap :=
+  match goal with
+  | |- context[foldMap (T := ?T) (M := ?M) (op := ?op) (unit := ?unit)] =>
+      rewrite foldMap_to_traverse1;
+      simplify_traverse;
+      repeat rewrite <- foldMap_to_traverse1;
+      simplify_foldMap_post
+  end.
+
+Lemma monoid_conjunction_rw:
+  forall (P1 P2: Prop),
+    monoid_op (Monoid_op := Monoid_op_and) P1 P2 = (P1 /\ P2).
+Proof.
+  reflexivity.
+Qed.
+
+Ltac simplify_monoid_conjunction :=
+  match goal with
+  | |- context[monoid_op (Monoid_op := Monoid_op_and) ?P1 ?P2] =>
+      rewrite monoid_conjunction_rw
+  end.
+
+Lemma monoid_append_rw:
+  forall {A} (l1 l2: list A),
+    monoid_op (Monoid_op := Monoid_op_list) l1 l2 = l1 ++ l2.
+Proof.
+  reflexivity.
+Qed.
+
+Lemma monoid_disjunction_rw:
+  forall (P1 P2: Prop),
+    monoid_op (Monoid_op := Monoid_op_or) P1 P2 = (P1 \/ P2).
+Proof.
+  reflexivity.
+Qed.
+
+Ltac simplify_monoid_disjunction :=
+  match goal with
+  | |- context[monoid_op (Monoid_op := Monoid_op_or) ?P1 ?P2] =>
+      rewrite monoid_disjunction_rw
+  end.
+
+Ltac simplify_monoid_append :=
+  rewrite monoid_append_rw.
+
+Lemma monoid_subset_rw:
+  forall {A} (l1 l2: subset A),
+    monoid_op (Monoid_op := Monoid_op_subset) l1 l2 = l1 ∪ l2.
+Proof.
+  reflexivity.
+Qed.
+
+Ltac simplify_monoid_subset :=
+  rewrite monoid_subset_rw.
+
+Ltac simplify_tolist :=
+  match goal with
+  | |- context[tolist (F := ?T) ?t] =>
+      rewrite (tolist_to_foldMap (T := T));
+      simplify_foldMap;
+      repeat rewrite <- (tolist_to_foldMap (T := T));
+      repeat simplify_monoid_append
+  end.
+
+Ltac simplify_tosubset :=
+  match goal with
+  | |- context[tosubset (F := ?T) (A := ?A) ?t] =>
+      rewrite (tosubset_to_foldMap (T := T) A);
+      simplify_foldMap;
+      repeat rewrite <- (tosubset_to_foldMap (T := T));
+      repeat simplify_monoid_subset
+  end;
+  (* This should only be necessary after binddt (ret x)) *)
+  try match goal with
+  | |- context[ret (T := ?T) (Return := Return_subset) ?a] =>
+      unfold_ops @Return_subset
+    end.
+
+Ltac simplify_toctxset :=
+  match goal with
+  | |- context[toctxset (F := ?T) ?t] =>
+      rewrite (toctxset_to_foldMapd (T := T) t);
+      simplify_foldMapd;
+      repeat rewrite <- (toctxset_to_foldMapd (T := T));
+      repeat simplify_monoid_subset
+  end;
+  (* This should only be necessary after binddt (ret x)) *)
+  try match goal with
+  | |- context[ret (T := ?T) (Return := Return_ctxset) ?a] =>
+      unfold_ops @Return_ctxset
+    end.
+
+Ltac simplify_element_of :=
+  match goal with
+  | |- context[element_of (F := ?T) (A := ?A) ?t] =>
+      rewrite (element_of_to_foldMap (T := T) A t);
+      simplify_foldMap;
+      repeat rewrite <- (element_of_to_foldMap (T := T));
+      repeat simplify_monoid_disjunction
+  end.
+
+Lemma simplify_singleton_ctx_S_preincr: forall {A} (a: A),
+  forall n, {{(S n, a)}} ⦿ 1 = {{(n, a)}}.
+Proof.
+  intros. ext [depth i]. cbv.
+  propext; do 2 rewrite pair_equal_spec; intuition.
+Qed.
+
+Lemma simplify_singleton_ctx_0_preincr: forall {A} (a: A),
+    {{(0, a)}} ⦿ 1 = const False.
+Proof.
+  intros. ext [depth i]. cbv.
+  propext; rewrite pair_equal_spec; intuition.
+Qed.
+
+Lemma simplify_singleton_ctx_preincr: forall {A} (a: A) n,
+    n > 1 ->
+    {{(n, a)}} ⦿ 1 = {{(n - 1, a)}}.
+Proof.
+  intros. ext [depth i].
+  unfold preincr, incr, compose.
+  simpl_subset. propext;
+    do 2 rewrite pair_equal_spec;
+    unfold_ops @Monoid_op_plus;
+    intuition.
+Qed.
+
+Ltac simplify_singleton_ctx_under_binder :=
+  match goal with
+  | |- context[{{?p}} ⦿ 1] =>
+      rewrite simplify_singleton_ctx_S_preincr
+  | |- context[{{(0, ?l)}} ⦿ 1] =>
+      rewrite simplify_singleton_ctx_0_preincr
+  end.
+
+Ltac simplify_element_ctx_of :=
+  match goal with
+  | |- context[element_ctx_of (T := ?T) (A := ?A) ?p] =>
+      rewrite (element_ctx_of_to_foldMapd (T := T) A p);
+      simplify_foldMapd;
+      try simplify_singleton_ctx_under_binder;
+      repeat rewrite <- (element_ctx_of_to_foldMapd (T := T));
+      repeat simplify_monoid_disjunction
+  end;
+  (* This should only be necessary after binddt (ret x)) *)
+  simpl_subset;
+  try rewrite pair_equal_spec.
+
+Ltac simplify_Forall_ctx :=
+  rewrite Forall_ctx_to_foldMapd;
+  simplify_foldMapd;
+  repeat rewrite <- Forall_ctx_to_foldMapd;
+  repeat simplify_monoid_conjunction.
+
+Ltac simplify_lc_loc_under_binder :=
+  match goal with
+  | |- context[lc_loc ?n ⦿ 1] =>
+      rewrite lc_loc_S
+  | |- context[lc_loc ?n ⦿ ?m] =>
+      rewrite lc_loc_preincr
+  end.
+
+Ltac simplify_lc_loc_leaf :=
+  match goal with
+  | |- context[lc_loc ?n (?w, Fr ?x)] =>
+      rewrite lc_loc_Fr
+  | |- context[lc_loc 0 (0, Bd ?b)] =>
+      rewrite lc_loc_00Bd
+  | |- context[lc_loc 0 (?w, Bd ?b)] =>
+      rewrite lc_loc_0Bd
+  | |- context[lc_loc ?n (?w, Bd ?b)] =>
+      rewrite lc_loc_nBd
+  end.
+
+Ltac simplify_arithmetic :=
+  match goal with
+  | |- context[(?x + 0)%nat] =>
+      replace (x + 0)%nat with x by lia
+  | |- context[(0 + ?x)%nat] =>
+      replace (0 + x)%nat with x by lia
+  end.
+
+Ltac simplify_LC :=
+  repeat change (LC ?t) with (LCn 0 t);
+  rewrite LCn_spec;
+  simplify_Forall_ctx;
+  repeat simplify_lc_loc_under_binder;
+  ( unfold_ops @Monoid_op_plus @Monoid_unit_zero;
+    try simplify_lc_loc_leaf;
+    repeat simplify_arithmetic);
+  (* ^ This should really only apply at (ret) *)
+  repeat rewrite <- LCn_spec;
+  repeat change (LCn 0 ?t) with (LC t).
+
+
+Ltac simplify_free_loc :=
+  match goal with
+  | |- context[free_loc ?v] =>
+      let e := constr:(free_loc v)in
+      let e' := eval cbn in e in
+        change e with e' in *
+  end.
+
+Ltac simplify_free :=
+  unfold free;
+  simplify_foldMap;
+  (* ^^ this exposes ● with lists *)
+  repeat simplify_monoid_append;
+  repeat change (foldMap free_loc ?t) with (free t);
+  repeat simplify_free_loc.
+
+Ltac simplify_FV :=
+  unfold FV;
+  simplify_free;
+  autorewrite with tea_rw_atoms.
+
+Ltac simplify_open :=
+  unfold open;
+  simplify_bindd;
+  repeat match goal with
+  | |- context[bindd (open_loc ?u) ?t] =>
+      try change (bindd (open_loc u) t) with (open u t)
+    end.
+
+Ltac simplify_subst :=
+  unfold subst;
+  simplify_bind;
+  repeat match goal with
+  | |- context[bind (subst_loc ?x ?u) ?t] =>
+      try change (bind (subst_loc x u) t) with (subst x u t)
+  end.
+
+Ltac simplify_derived_operations :=
+  match goal with
+  | |- context[tolist ?t] =>
+      debug "";
+      simplify_tolist
+  | |- context[element_ctx_of ?x ?t] =>
+      debug "";
+      simplify_element_ctx_of
+  | |- context[toctxset ?t] =>
+      debug "";
+      simplify_toctxset
+  | |- context[element_of ?x ?t] =>
+      debug "";
+      simplify_element_of
+  | |- context[tosubset ?t] =>
+      debug "";
+      simplify_tosubset
+  end.
+
+Ltac simplify_LN :=
+  match goal with
+  | |- context[LCn ?t] =>
+      debug "";
+      simplify_LC
+  | |- context[LC ?t] =>
+      debug "";
+      simplify_LC
+  | |- context[free ?t] =>
+      debug "";
+      simplify_free
+  | |- context[open ?t] =>
+      debug "";
+      simplify_open
+  end.
+
+Ltac simplify :=
+  repeat simplify_LN;
+  repeat simplify_derived_operations;
+  simpl_list.
+
+(** ** Rewriting lemmas for <<LC>> *)
+(******************************************************************************)
+Theorem term_lcn11 : forall (n : nat) (m : nat),
+    LCn m (tvar (Bd n)) <-> n < m.
+Proof.
+  intros. simplify_LC. reflexivity.
+Qed.
+
+Theorem term_lcn12 : forall (x : atom) (m : nat),
+    LCn m (tvar (Fr x)) <-> True.
+Proof.
+  intros. simplify_LN. reflexivity.
+Qed.
+
+Theorem term_lcn2 : forall (X : typ) (t : term LN) (m : nat),
+    LCn m (lam X t) <-> LCn (S m) t.
+Proof.
+  intros. simplify_LN. reflexivity.
+Qed.
+
+Theorem term_lcn3 : forall (t1 t2 : term LN) (m : nat),
+    LCn m ([t1]@[t2]) <->
+      LCn m t1 /\ LCn m t2.
+Proof.
+  intros. simplify_LN. reflexivity.
+Qed.
+
+Theorem term_lc11 : forall (n : nat),
+    LC (tvar (Bd n)) <-> False.
+Proof.
+  intros. simplify_LN. lia.
+Qed.
+
+Theorem term_lc12 : forall (x : atom),
+    LC (tvar (Fr x)) <-> True.
+Proof.
+  intros. simplify_LN. reflexivity.
+Qed.
+
+Theorem term_lc2 : forall (X : typ) (t : term LN),
+    LC (lam X t) <-> LCn 1 t.
+Proof.
+  intros. simplify_LN. reflexivity.
+Qed.
+
+Theorem term_lc3 : forall (t1 t2 : term LN),
+    LC ([t1]@[t2]) <-> LC t1 /\ LC t2.
+Proof.
+  intros. simplify_LN. reflexivity.
+Qed.
 
 (** ** Rewriting lemmas for <<tolist>>, <<toset>>, <<∈>> *)
 (******************************************************************************)
@@ -15,46 +525,57 @@ Section term_container_rewrite.
   Variable
     (A : Type).
 
-  Definition tolist_tvar_rw1: forall (x: A),
-      tolist (tvar x) = [x] :=
-    ltac:(simplify).
+  Lemma tolist_tvar_rw1: forall (x: A),
+      tolist (tvar x) = [x].
+  Proof.
+    intros. simplify. reflexivity.
+  Qed.
 
-  Definition tolist_term_rw2: forall (X: typ) (t: term A),
-      tolist (lam X t) = tolist t :=
-    ltac:(simplify).
+  Lemma tolist_term_rw2: forall (X: typ) (t: term A),
+      tolist (lam X t) = tolist t.
+  Proof.
+    intros. simplify. reflexivity.
+  Qed.
 
-  Definition tolist_term_rw3: forall (t1 t2: term A),
-      tolist (app t1 t2) = tolist t1 ++ tolist t2 :=
-    ltac:(simplify).
+  Lemma tolist_term_rw3: forall (t1 t2: term A),
+      tolist (app t1 t2) = tolist t1 ++ tolist t2.
+  Proof.
+    intros. simplify. reflexivity.
+  Qed.
+  Lemma toset_tvar_rw1: forall (x: A),
+      tosubset (tvar x) = {{x}}.
+  Proof.
+    intros. simplify. reflexivity.
+  Qed.
 
-  Definition toset_tvar_rw1: forall (x: A),
-      tosubset (tvar x) = {{x}}
-    := ltac:(simplify).
+  Lemma toset_term_rw2: forall (X: typ) (t: term A),
+      tosubset (lam X t) = tosubset t.
+  Proof.
+    intros. simplify_tosubset. reflexivity.
+  Qed.
 
-  Definition toset_term_rw2: forall (X: typ) (t: term A),
-      tosubset (lam X t) = tosubset t
-    := ltac:(simplify).
-
-  Definition toset_term_rw3: forall (t1 t2: term A),
-      tosubset (app t1 t2) = tosubset t1 ∪ tosubset t2
-    := ltac:(simplify).
+  Lemma toset_term_rw3: forall (t1 t2: term A),
+      tosubset (app t1 t2) = tosubset t1 ∪ tosubset t2.
+  Proof.
+    intros. simplify. reflexivity.
+  Qed.
 
   Lemma in_term_rw1: forall (x y: A),
       x ∈ tvar y <-> x = y.
   Proof.
-    simplify.
+    intros. simplify. reflexivity.
   Qed.
 
   Lemma in_term_rw2: forall (y: A) (X: typ) (t: term A),
-    y ∈ (lam X t) <-> y ∈ t.
+      y ∈ (lam X t) <-> y ∈ t.
   Proof.
-    simplify.
+    intros. simplify. reflexivity.
   Qed.
 
   Lemma in_term_3: forall (t1 t2: term A) (y: A),
       y ∈ (app t1 t2) <-> y ∈ t1 \/ y ∈ t2.
   Proof.
-    simplify.
+    intros. simplify. reflexivity.
   Qed.
 
 End term_container_rewrite.
@@ -66,86 +587,102 @@ Section term_free_rewrite.
   Variable (A : Type).
 
   Definition term_free11 : forall (b : nat),
-      free (tvar (Bd b)) = []
-    := ltac:(simplify).
+      free (tvar (Bd b)) = [].
+  Proof.
+    intros. simplify_LN. reflexivity.
+  Qed.
 
   Definition term_in_free11 : forall (b : nat) (x : atom),
-      x ∈ free (tvar (Bd b)) <-> False
-    := ltac:(simplify).
+      x ∈ free (tvar (Bd b)) <-> False.
+  Proof.
+    intros. simplify_LN. reflexivity.
+  Qed.
 
   Definition term_free12 : forall (y : atom),
-      free (tvar (Fr y)) = [y]
-    := ltac:(simplify).
+      free (tvar (Fr y)) = [y].
+  Proof.
+    intros. simplify_LN. reflexivity.
+  Qed.
 
   Definition term_in_free12 : forall (y : atom) (x : atom),
-      x ∈ free (tvar (Fr y)) <-> x = y
-    := ltac:(simplify).
+      x ∈ free (tvar (Fr y)) <-> x = y.
+  Proof.
+    intros. simplify. reflexivity.
+  Qed.
 
   Definition term_free2 : forall (t : term LN) (X : typ),
-      free (lam X t) = free t
-    := ltac:(simplify).
+      free (lam X t) = free t.
+  Proof.
+    intros. simplify_LN. reflexivity.
+  Qed.
 
   Definition term_in_free2 : forall (x : atom) (t : term LN) (X : typ),
-      x ∈ free (lam X t) <-> x ∈ free t
-    := ltac:(simplify).
+      x ∈ free (lam X t) <-> x ∈ free t.
+  Proof.
+    intros. simplify. reflexivity.
+  Qed.
 
   Definition term_free3 : forall (x : atom) (t1 t2 : term LN),
-      free (app t1 t2) = free t1 ++ free t2
-    := ltac:(simplify).
+      free (app t1 t2) = free t1 ++ free t2.
+  Proof.
+    intros. simplify. reflexivity.
+  Qed.
 
   Definition term_in_free3 : forall (x : atom) (t1 t2 : term LN),
-      x ∈ free (app t1 t2) <-> x ∈ free t1 \/ x ∈ free t2
-    := ltac:(simplify).
-
-  Definition term_in_freeset11 : forall (b : nat) (x : atom),
-      AtomSet.In x (freeset (tvar (Bd b))) <-> False.
+      x ∈ free (app t1 t2) <-> x ∈ free t1 \/ x ∈ free t2.
   Proof.
-    try simplify.
-  Admitted.
-
-  Definition term_in_freeset12 : forall (y : atom) (x : atom),
-      AtomSet.In x (freeset (tvar (Fr y))) <-> x = y.
-  Proof.
-    simplify.
+    intros. simplify. reflexivity.
   Qed.
 
-  Lemma term_in_freeset2 : forall (x : atom) (t : term LN) (X : typ),
-      AtomSet.In x (freeset (lam X t)) <-> AtomSet.In x (freeset t).
+  Definition term_in_FV11 : forall (b : nat) (x : atom),
+      x `in` FV (tvar (Bd b)) <-> False.
   Proof.
-    simplify.
+    intros. simplify_FV. reflexivity.
   Qed.
 
-  Lemma term_in_freeset3 : forall (x : atom) (t1 t2 : term LN),
-      AtomSet.In x (freeset (app t1 t2)) <->
-        AtomSet.In x (freeset t1) \/ AtomSet.In x (freeset t2).
+  Definition term_in_FV12 : forall (y : atom) (x : atom),
+      AtomSet.In x (FV (tvar (Fr y))) <-> x = y.
   Proof.
-    simplify.
+    intros. simplify_FV. reflexivity.
+  Qed.
+
+  Lemma term_in_FV2 : forall (x : atom) (t : term LN) (X : typ),
+      AtomSet.In x (FV (lam X t)) <-> AtomSet.In x (FV t).
+  Proof.
+    intros. simplify_FV. reflexivity.
+  Qed.
+
+  Lemma term_in_FV3 : forall (x : atom) (t1 t2 : term LN),
+      AtomSet.In x (FV (app t1 t2)) <->
+        AtomSet.In x (FV t1) \/ AtomSet.In x (FV t2).
+  Proof.
+    intros. simplify_FV. reflexivity.
   Qed.
 
   Open Scope set_scope.
 
-  Lemma term_freeset11 : forall (b : nat) (x : atom),
-      freeset (tvar (Bd b)) [=] ∅.
+  Lemma term_FV11 : forall (b : nat) (x : atom),
+      FV (tvar (Bd b)) [=] ∅.
   Proof.
-    intros. fsetdec.
+    intros. simplify_FV. fsetdec.
   Qed.
 
-  Lemma term_freeset12 : forall (y : atom),
-      freeset (tvar (Fr y)) [=] {{ y }}.
+  Lemma term_FV12 : forall (y : atom),
+      FV (tvar (Fr y)) [=] {{ y }}.
   Proof.
-    simplify.
+    intros. simplify_FV. fsetdec.
   Qed.
 
-  Lemma term_freeset2 : forall (t : term LN) (X : typ),
-      freeset (lam X t) [=] freeset t.
+  Lemma term_FV2 : forall (t : term LN) (X : typ),
+      FV (lam X t) [=] FV t.
   Proof.
-    simplify.
+    intros. simplify_FV. fsetdec.
   Qed.
 
-  Lemma term_freeset3 : forall (t1 t2 : term LN),
-      freeset (app t1 t2) [=] freeset t1 ∪ freeset t2.
+  Lemma term_FV3 : forall (t1 t2 : term LN),
+      FV (app t1 t2) [=] FV t1 ∪ FV t2.
   Proof.
-    simplify.
+    intros. simplify_FV. fsetdec.
   Qed.
 
 End term_free_rewrite.
@@ -159,19 +696,19 @@ Section term_foldMapd_rewrite.
   Lemma term_foldMapd1 : forall (a : A),
       foldMapd f (tvar a) = f (Ƶ, a).
   Proof.
-    simplify.
+    intros. simplify_foldMapd. reflexivity.
   Qed.
 
   Lemma term_foldMapd2 : forall X (t : term A),
       foldMapd f (λ X t) = foldMapd (f ⦿ 1) t.
   Proof.
-    simplify.
+    intros. simplify_foldMapd. reflexivity.
   Qed.
 
   Lemma term_foldMapd3 : forall (t1 t2 : term A),
       foldMapd f ([t1]@[t2]) = foldMapd f t1 ● foldMapd f t2.
   Proof.
-    simplify.
+    intros. simplify_foldMapd. reflexivity.
   Qed.
 
 End term_foldMapd_rewrite.
@@ -183,103 +720,36 @@ Section term_ind_rewrite.
   Lemma term_ind1 : forall (l1 l2 : LN) (n : nat),
       (n, l1) ∈d (tvar l2) <-> n = Ƶ /\ l1 = l2.
   Proof.
-    simplify.
+    intros. simplify_element_ctx_of. reflexivity.
   Qed.
+
+  Ltac print_goal := match goal with
+  | |- ?g => idtac g (* prints goal *)
+  end.
+
 
   Lemma term_ind2 : forall (t : term LN) (l : LN) (n : nat) (X : typ),
       (n, l) ∈d t = (S n, l) ∈d (λ X t).
   Proof.
-    simplify.
+    intros. simplify_element_ctx_of. reflexivity.
   Qed.
 
   Lemma term_ind2_nZ : forall (t : term LN) (l : LN) (n : nat) (X : typ),
-      (n, l) ∈d (λ X t) -> (n <> 0).
+      (n, l) ∈d (λ X t) -> n <> 0.
   Proof.
     introv.
-    Ltac simplify_pass1 :=
-      simplify_pass1_with_simplify_binddt term simplify_binddt_term_lazy.
-    repeat simplify_pass1.
-    repeat simplify_pass2.
-    assert (Hgt: 1 > 0) by lia; generalize dependent Hgt.
-    generalize 1 as m.
-    induction t;
-      intros m Hgt;
-      repeat simplify_pass1;
-      repeat simplify_pass2.
-    - unfold preincr, compose, incr; cbn.
-      rewrite pair_equal_spec.
-      change (?m ● ?x) with (m + x)%nat. lia.
-    - rewrite preincr_preincr.
-      intro hyp.
-      eapply IHt.
-      2: eauto.
-      change (?m ● ?x) with (m + x)%nat.
-      lia.
-    - intros [hyp|hyp]; eauto.
+    destruct n.
+    - simplify_element_ctx_of.
+      rewrite exists_false_false.
+      easy.
+    - simplify_element_ctx_of.
+      easy.
   Qed.
-
-  Lemma term_ind2_nZ2: forall t n l,
-      (@binddt nat term term Binddt_STLC (@const Type Type Prop)
-        (@Map_const Prop) (@Pure_const Prop False) (@Mult_const Prop or) LN False
-        (eq (n, l) ⦿ 1) t) -> n <> 0.
-  Proof.
-    introv.
-    assert (Hgt: 1 > 0) by lia; generalize dependent Hgt.
-    generalize 1 as m.
-    induction t;
-      intros m Hgt;
-      simplify_pass1;
-      repeat simplify_pass2.
-    - unfold preincr, compose, incr; cbn.
-      rewrite pair_equal_spec.
-      change (?m ● ?x) with (m + x)%nat.
-      lia.
-    - rewrite preincr_preincr.
-      intro hyp.
-      eapply IHt.
-      2: eauto.
-      change (?m ● ?x) with (m + x)%nat.
-      lia.
-    - intros [hyp|hyp]; eauto.
-  Qed.
-
-  (*
-  Lemma term_ind2_alt : forall (t : term LN) (l : LN) (n : nat) (X : typ),
-      (n, l) ∈d (λ X t) = ((n - 1, l) ∈d t /\ n <> 0).
-  Proof.
-    intros.
-    propext.
-    - intro.
-      specialize (term_ind2_nZ2 t l H).
-      intro. destruct n.
-      + false.
-      + replace (S n - 1) with n by lia.
-        apply term_ind2 in H.
-    do 2 rewrite ind_to_foldMapd.
-    simplify.
-    simplify.
-    simplify.
-    simplify.
-    simplify.
-    simplify.
-    simplify.
-    simplify.
-    simplify.
-                  .
-
-    - intro. destruct H as [H H'].
-      destruct n.
-      + false.
-      + rewrite <- eq_pair_preincr.
-        replace (S n - 1) with n in H by lia.
-        assumption.
-  Qed.
-  *)
 
   Lemma term_ind3 : forall (t1 t2 : term LN) (n : nat) (l : LN),
       (n, l) ∈d ([t1]@[t2]) <-> (n, l) ∈d t1 \/ (n, l) ∈d t2.
   Proof.
-    simplify.
+    intros. simplify. reflexivity.
   Qed.
 
 End term_ind_rewrite.
@@ -287,17 +757,15 @@ End term_ind_rewrite.
 (** ** Rewriting lemmas for <<open>> *)
 (******************************************************************************)
 Lemma open_term_rw2: forall (t1 t2: term LN) u,
-    open u (app t1 t2) =
-      app (open u t1) (open u t2).
+    open u (app t1 t2) = app (open u t1) (open u t2).
 Proof.
-  simplify.
+  intros. simplify_open. reflexivity.
 Qed.
 
 Lemma open_term_rw3: forall τ (t: term LN) u,
-    open u (λ τ t) =
-      λ τ (bindd (open_loc u ⦿ 1) t).
+    open u (λ τ t) = λ τ (bindd (open_loc u ⦿ 1) t).
 Proof.
-  simplify.
+  intros. simplify_open. reflexivity.
 Qed.
 
 (** ** Rewriting lemmas for <<subst>> *)
@@ -306,63 +774,12 @@ Lemma subst_term_rw2: forall (t1 t2: term LN) x u,
     subst x u (app t1 t2) =
       app (subst x u t1) (subst x u t2).
 Proof.
-  simplify.
+  intros. simplify_subst. reflexivity.
 Qed.
 
 Lemma subst_term_rw3: forall τ (t: term LN) x u,
     subst x u (λ τ t) =
       λ τ (subst x u t).
 Proof.
-  simplify.
-Qed.
-
-(** ** Rewriting lemmas for <<locally_closed>> *)
-(******************************************************************************)
-Theorem term_lc_gap11 : forall (n : nat) (m : nat),
-    locally_closed_gap m (tvar (Bd n)) <-> n < m.
-Proof.
-  simplify.
-Qed.
-
-Theorem term_lc_gap12 : forall (x : atom) (m : nat),
-    locally_closed_gap m (tvar (Fr x)) <-> True.
-Proof.
-  simplify.
-Qed.
-
-Theorem term_lc_gap2 : forall (X : typ) (t : term LN) (m : nat),
-    locally_closed_gap m (lam X t) <-> locally_closed_gap (S m) t.
-Proof.
-  simplify.
-Qed.
-
-Theorem term_lc_gap3 : forall (t1 t2 : term LN) (m : nat),
-    locally_closed_gap m ([t1]@[t2]) <->
-      locally_closed_gap m t1 /\ locally_closed_gap m t2.
-Proof.
-  simplify.
-Qed.
-
-Theorem term_lc11 : forall (n : nat),
-    locally_closed (tvar (Bd n)) <-> False.
-Proof.
-  simplify.
-Qed.
-
-Theorem term_lc12 : forall (x : atom),
-    locally_closed (tvar (Fr x)) <-> True.
-Proof.
-  simplify.
-Qed.
-
-Theorem term_lc2 : forall (X : typ) (t : term LN),
-    locally_closed (lam X t) <-> locally_closed_gap 1 t.
-Proof.
-  simplify.
-Qed.
-
-Theorem term_lc3 : forall (t1 t2 : term LN),
-    locally_closed ([t1]@[t2]) <-> locally_closed t1 /\ locally_closed t2.
-Proof.
-  simplify.
+  intros. simplify_subst. reflexivity.
 Qed.
